Extend compartmentalized memory to Stacking
The Stacking proof is perhaps the most interesting part of the backend,
in particular because the separation invariants on memories need to be
handled with some care. A conjunct stating memory ownership is added
together with the usual compartment parameter. The new proof obligation
is solved then instead of relegated, so that the unnecessary section
variables and hypotheses can be removed once the section is closed to
avoid interfering with external users. Nonetheless, some hypothesis
renumbering derived from the new conjunct seems difficult to avoid.

A small number of subgoals, in particular variants of old goals rather
than new goals, need a bit more work than usual to close all the gaps.

backend/Stackingproof.v
@@ -156,9 +156,9 @@ Local Opaque Z.add Z.mul Z.divide.
 (** Accessing the stack frame using [load_stack] and [store_stack]. *)
 
 Lemma contains_get_stack:
-  forall spec m ty sp ofs,
-  m |= contains (chunk_of_type ty) sp ofs spec ->
-  exists v, load_stack m (Vptr sp Ptrofs.zero) ty (Ptrofs.repr ofs) = Some v /\ spec v.
+  forall spec m ty sp ofs cp,
+  m |= contains (chunk_of_type ty) sp ofs cp spec ->
+  exists v, load_stack m (Vptr sp Ptrofs.zero) ty (Ptrofs.repr ofs) cp = Some v /\ spec v.
 Proof.
   intros. unfold load_stack.
   replace (Val.offset_ptr (Vptr sp Ptrofs.zero) (Ptrofs.repr ofs)) with (Vptr sp (Ptrofs.repr ofs)).
@@ -167,20 +167,20 @@ Proof.
 Qed.
 
 Lemma hasvalue_get_stack:
-  forall ty m sp ofs v,
-  m |= hasvalue (chunk_of_type ty) sp ofs v ->
-  load_stack m (Vptr sp Ptrofs.zero) ty (Ptrofs.repr ofs) = Some v.
+  forall ty m sp ofs cp v,
+  m |= hasvalue (chunk_of_type ty) sp ofs cp v ->
+  load_stack m (Vptr sp Ptrofs.zero) ty (Ptrofs.repr ofs) cp = Some v.
 Proof.
   intros. exploit contains_get_stack; eauto. intros (v' & A & B). congruence.
 Qed.
 
 Lemma contains_set_stack:
-  forall (spec: val -> Prop) v spec1 m ty sp ofs P,
-  m |= contains (chunk_of_type ty) sp ofs spec1 ** P ->
+  forall (spec: val -> Prop) v spec1 m ty sp ofs cp P,
+  m |= contains (chunk_of_type ty) sp ofs cp spec1 ** P ->
   spec (Val.load_result (chunk_of_type ty) v) ->
   exists m',
-      store_stack m (Vptr sp Ptrofs.zero) ty (Ptrofs.repr ofs) v = Some m'
-  /\ m' |= contains (chunk_of_type ty) sp ofs spec ** P.
+      store_stack m (Vptr sp Ptrofs.zero) ty (Ptrofs.repr ofs) v cp = Some m'
+  /\ m' |= contains (chunk_of_type ty) sp ofs cp spec ** P.
 Proof.
   intros. unfold store_stack.
   replace (Val.offset_ptr (Vptr sp Ptrofs.zero) (Ptrofs.repr ofs)) with (Vptr sp (Ptrofs.repr ofs)).
@@ -197,12 +197,27 @@ Qed.
   reason about the values of [Local] slots, the other about the values of
   [Outgoing] slots. *)
 
-Program Definition contains_locations (j: meminj) (sp: block) (pos bound: Z) (sl: slot) (ls: locset) : massert := {|
+(* RB: NOTE: Adding compartment parameter here with corresponding
+   [Mem.own_block] conjunct to link premise and conclusion, where the
+   compartment is strictly needed.
+
+   It might be interesting to derive [Mem.own_block] from other permissions,
+   however for now exposing the new dependencies as parameters seems enough.
+
+   Unfortunately, the added conjunct modifies automatically generated names of
+   related hypotheses in proofs below, and there is no clear way to avoid this.
+
+   There is a new proof obligation that we need to solve to avoid unnecessary
+   section when we use the assertion later.
+
+   The documentation above (and for related assertions) needs to be amended. *)
+Program Definition contains_locations (j: meminj) (sp: block) (pos bound: Z) (sl: slot) (ls: locset) (cp: compartment) : massert := {|
   m_pred := fun m =>
     (8 | pos) /\ 0 <= pos /\ pos + 4 * bound <= Ptrofs.modulus /\
     Mem.range_perm m sp pos (pos + 4 * bound) Cur Freeable /\
+    Mem.own_block m sp cp /\
     forall ofs ty, 0 <= ofs -> ofs + typesize ty <= bound -> (typealign ty | ofs) ->
-    exists v, Mem.load (chunk_of_type ty) m sp (pos + 4 * ofs) = Some v
+    exists v, Mem.load (chunk_of_type ty) m sp (pos + 4 * ofs) cp = Some v
            /\ Val.inject j (ls (S sl ofs ty)) v;
   m_footprint := fun b ofs =>
     b = sp /\ pos <= ofs < pos + 4 * bound
@@ -210,9 +225,12 @@ Program Definition contains_locations (j: meminj) (sp: block) (pos bound: Z) (sl
 Next Obligation.
   intuition auto.
 - red; intros. eapply Mem.perm_unchanged_on; eauto. simpl; auto.
-- exploit H4; eauto. intros (v & A & B). exists v; split; auto.
+- apply (Mem.unchanged_on_own _ _ _ H0).
+  + eapply Mem.own_block_valid_block; now eauto.
+  + assumption.
+- exploit H5; eauto. intros (v & A & B). exists v; split; auto.
   eapply Mem.load_unchanged_on; eauto.
-  simpl; intros. rewrite size_type_chunk, typesize_typesize in H8.
+  simpl; intros. rewrite size_type_chunk, typesize_typesize in H9.
   split; auto. omega.
 Qed.
 Next Obligation.
@@ -220,45 +238,48 @@ Next Obligation.
 Qed.
 
 Remark valid_access_location:
-  forall m sp pos bound ofs ty p,
+  forall m sp pos bound cp ofs ty p,
   (8 | pos) ->
   Mem.range_perm m sp pos (pos + 4 * bound) Cur Freeable ->
+  Mem.own_block m sp cp ->
   0 <= ofs -> ofs + typesize ty <= bound -> (typealign ty | ofs) ->
-  Mem.valid_access m (chunk_of_type ty) sp (pos + 4 * ofs) p.
+  Mem.valid_access m (chunk_of_type ty) sp (pos + 4 * ofs) p cp.
 Proof.
   intros; split.
 - red; intros. apply Mem.perm_implies with Freeable; auto with mem.
-  apply H0. rewrite size_type_chunk, typesize_typesize in H4. omega.
-- rewrite align_type_chunk. apply Z.divide_add_r.
+  apply H0. rewrite size_type_chunk, typesize_typesize in H5. omega.
+- split. admit. (* RB: NOTE: New own_block subgoal *)
+  rewrite align_type_chunk. apply Z.divide_add_r.
   apply Z.divide_trans with 8; auto.
   exists (8 / (4 * typealign ty)); destruct ty; reflexivity.
   apply Z.mul_divide_mono_l. auto.
-Qed.
+(* Qed. *)
+Admitted.
 
 Lemma get_location:
-  forall m j sp pos bound sl ls ofs ty,
-  m |= contains_locations j sp pos bound sl ls ->
+  forall m j sp pos bound sl ls cp ofs ty,
+  m |= contains_locations j sp pos bound sl ls cp ->
   0 <= ofs -> ofs + typesize ty <= bound -> (typealign ty | ofs) ->
   exists v,
-     load_stack m (Vptr sp Ptrofs.zero) ty (Ptrofs.repr (pos + 4 * ofs)) = Some v
+     load_stack m (Vptr sp Ptrofs.zero) ty (Ptrofs.repr (pos + 4 * ofs)) cp = Some v
   /\ Val.inject j (ls (S sl ofs ty)) v.
 Proof.
-  intros. destruct H as (D & E & F & G & H).
+  intros. destruct H as (D & E & F & G & [H' H]).
   exploit H; eauto. intros (v & U & V). exists v; split; auto.
   unfold load_stack; simpl. rewrite Ptrofs.add_zero_l, Ptrofs.unsigned_repr; auto.
   unfold Ptrofs.max_unsigned. generalize (typesize_pos ty). omega.
 Qed.
 
 Lemma set_location:
-  forall m j sp pos bound sl ls P ofs ty v v',
-  m |= contains_locations j sp pos bound sl ls ** P ->
+  forall m j sp pos bound sl cp ls P ofs ty v v',
+  m |= contains_locations j sp pos bound sl ls cp ** P ->
   0 <= ofs -> ofs + typesize ty <= bound -> (typealign ty | ofs) ->
   Val.inject j v v' ->
   exists m',
-     store_stack m (Vptr sp Ptrofs.zero) ty (Ptrofs.repr (pos + 4 * ofs)) v' = Some m'
-  /\ m' |= contains_locations j sp pos bound sl (Locmap.set (S sl ofs ty) v ls) ** P.
+     store_stack m (Vptr sp Ptrofs.zero) ty (Ptrofs.repr (pos + 4 * ofs)) v' cp = Some m'
+  /\ m' |= contains_locations j sp pos bound sl (Locmap.set (S sl ofs ty) v ls) cp ** P.
 Proof.
-  intros. destruct H as (A & B & C). destruct A as (D & E & F & G & H).
+  intros. destruct H as (A & B & C). destruct A as (D & E & F & G & [H' H]).
   edestruct Mem.valid_access_store as [m' STORE].
   eapply valid_access_location; eauto.
   assert (PERM: Mem.range_perm m' sp pos (pos + 4 * bound) Cur Freeable).
@@ -267,6 +288,7 @@ Proof.
 - unfold store_stack; simpl. rewrite Ptrofs.add_zero_l, Ptrofs.unsigned_repr; eauto.
   unfold Ptrofs.max_unsigned. generalize (typesize_pos ty). omega.
 - simpl. intuition auto.
++ admit. (* RB: NOTE: New own_block subgoal *)
 + unfold Locmap.set.
   destruct (Loc.eq (S sl ofs ty) (S sl ofs0 ty0)); [|destruct (Loc.diff_dec (S sl ofs ty) (S sl ofs0 ty0))].
 * (* same location *)
@@ -279,51 +301,58 @@ Proof.
   rewrite <- X; eapply Mem.load_store_other; eauto.
   destruct d. congruence. right. rewrite ! size_type_chunk, ! typesize_typesize. omega.
 * (* overlapping locations *)
-  destruct (Mem.valid_access_load m' (chunk_of_type ty0) sp (pos + 4 * ofs0)) as [v'' LOAD].
+  destruct (Mem.valid_access_load m' (chunk_of_type ty0) sp (pos + 4 * ofs0) cp) as [v'' LOAD].
   apply Mem.valid_access_implies with Writable; auto with mem.
   eapply valid_access_location; eauto.
+  admit. (* RB: NOTE: New own_block subgoal *)
   exists v''; auto.
 + apply (m_invar P) with m; auto.
   eapply Mem.store_unchanged_on; eauto.
   intros i; rewrite size_type_chunk, typesize_typesize. intros; red; intros.
   eelim C; eauto. simpl. split; auto. omega.
-Qed.
+(* Qed. *)
+Admitted.
 
 Lemma initial_locations:
-  forall j sp pos bound P sl ls m,
+  forall j sp pos bound P sl ls cp m,
   m |= range sp pos (pos + 4 * bound) ** P ->
   (8 | pos) ->
   (forall ofs ty, ls (S sl ofs ty) = Vundef) ->
-  m |= contains_locations j sp pos bound sl ls ** P.
+  m |= contains_locations j sp pos bound sl ls cp ** P.
 Proof.
   intros. destruct H as (A & B & C). destruct A as (D & E & F). split.
 - simpl; intuition auto. red; intros; eauto with mem.
-  destruct (Mem.valid_access_load m (chunk_of_type ty) sp (pos + 4 * ofs)) as [v LOAD].
-  eapply valid_access_location; eauto.
-  red; intros; eauto with mem.
+  admit. (* RB: NOTE: New own_block subgoal *)
+  destruct (Mem.valid_access_load m (chunk_of_type ty) sp (pos + 4 * ofs) cp) as [v LOAD].
+  admit. (* RB: NOTE: This subgoal needs fixing *)
+  (* eapply valid_access_location; eauto. *)
+  (* red; intros; eauto with mem. *)
   exists v; split; auto. rewrite H1; auto.
 - split; assumption.
-Qed.
+(* Qed. *)
+Admitted.
 
 Lemma contains_locations_exten:
-  forall ls ls' j sp pos bound sl,
+  forall ls ls' j sp pos bound sl cp,
   (forall ofs ty, Val.lessdef (ls' (S sl ofs ty)) (ls (S sl ofs ty))) ->
-  massert_imp (contains_locations j sp pos bound sl ls)
-              (contains_locations j sp pos bound sl ls').
+  massert_imp (contains_locations j sp pos bound sl ls cp)
+              (contains_locations j sp pos bound sl ls' cp).
 Proof.
   intros; split; simpl; intros; auto.
-  intuition auto. exploit H5; eauto. intros (v & A & B). exists v; split; auto. 
+  (* RB: NOTE: Try to avoid renumbering when using these definitions,
+     also above. *)
+  intuition auto. exploit H6; eauto. intros (v & A & B). exists v; split; auto.
   specialize (H ofs ty). inv H. congruence. auto. 
 Qed.
 
 Lemma contains_locations_incr:
-  forall j j' sp pos bound sl ls,
+  forall j j' sp pos bound sl ls cp,
   inject_incr j j' ->
-  massert_imp (contains_locations j sp pos bound sl ls)
-              (contains_locations j' sp pos bound sl ls).
+  massert_imp (contains_locations j sp pos bound sl ls cp)
+              (contains_locations j' sp pos bound sl ls cp).
 Proof.
   intros; split; simpl; intros; auto.
-  intuition auto. exploit H5; eauto. intros (v & A & B). exists v; eauto.
+  intuition auto. exploit H6; eauto. intros (v & A & B). exists v; eauto.
 Qed.
 
 (** [contains_callee_saves j sp pos rl ls] is a memory assertion that holds
@@ -332,23 +361,23 @@ Qed.
   up to the memory injection [j].  The memory layout of the registers in [rl]
   is the same as that implemented by [save_callee_save_rec]. *)
 
-Fixpoint contains_callee_saves (j: meminj) (sp: block) (pos: Z) (rl: list mreg) (ls: locset) : massert :=
+Fixpoint contains_callee_saves (j: meminj) (sp: block) (pos: Z) (rl: list mreg) (ls: locset) (cp: compartment) : massert :=
   match rl with
   | nil => pure True
   | r :: rl =>
       let ty := mreg_type r in
       let sz := AST.typesize ty in
       let pos1 := align pos sz in
-      contains (chunk_of_type ty) sp pos1 (fun v => Val.inject j (ls (R r)) v)
-      ** contains_callee_saves j sp (pos1 + sz) rl ls
+      contains (chunk_of_type ty) sp pos1 cp (fun v => Val.inject j (ls (R r)) v)
+      ** contains_callee_saves j sp (pos1 + sz) rl ls cp
   end.
 
 Lemma contains_callee_saves_incr:
   forall j j' sp ls,
   inject_incr j j' ->
-  forall rl pos,
-  massert_imp (contains_callee_saves j sp pos rl ls)
-              (contains_callee_saves j' sp pos rl ls).
+  forall rl pos cp,
+  massert_imp (contains_callee_saves j sp pos rl ls cp)
+              (contains_callee_saves j' sp pos rl ls cp).
 Proof.
   induction rl as [ | r1 rl]; simpl; intros.
 - reflexivity.
@@ -356,10 +385,10 @@ Proof.
 Qed.
 
 Lemma contains_callee_saves_exten:
-  forall j sp ls ls' rl pos,
+  forall j sp ls ls' rl pos cp,
   (forall r, In r rl -> ls' (R r) = ls (R r)) ->
-  massert_eqv (contains_callee_saves j sp pos rl ls)
-              (contains_callee_saves j sp pos rl ls').
+  massert_eqv (contains_callee_saves j sp pos rl ls cp)
+              (contains_callee_saves j sp pos rl ls' cp).
 Proof.
   induction rl as [ | r1 rl]; simpl; intros.
 - reflexivity.
@@ -379,26 +408,28 @@ In addition, we use a nonseparating conjunction to record the fact that
 we have full access rights on the stack frame, except the part that
 represents the Linear stack data. *)
 
-Definition frame_contents_1 (j: meminj) (sp: block) (ls ls0: locset) (parent retaddr: val) :=
-    contains_locations j sp fe.(fe_ofs_local) b.(bound_local) Local ls
- ** contains_locations j sp fe_ofs_arg b.(bound_outgoing) Outgoing ls
- ** hasvalue Mptr sp fe.(fe_ofs_link) parent
- ** hasvalue Mptr sp fe.(fe_ofs_retaddr) retaddr
- ** contains_callee_saves j sp fe.(fe_ofs_callee_save) b.(used_callee_save) ls0.
+Definition frame_contents_1 (j: meminj) (sp: block) (ls ls0: locset) (parent retaddr: val) (cp: compartment) :=
+  (* let cp := default_compartment in *)
+    contains_locations j sp fe.(fe_ofs_local) b.(bound_local) Local ls cp
+ ** contains_locations j sp fe_ofs_arg b.(bound_outgoing) Outgoing ls cp
+ ** hasvalue Mptr sp fe.(fe_ofs_link) cp parent
+ ** hasvalue Mptr sp fe.(fe_ofs_retaddr) cp retaddr
+ ** contains_callee_saves j sp fe.(fe_ofs_callee_save) b.(used_callee_save) ls0 cp.
 
-Definition frame_contents (j: meminj) (sp: block) (ls ls0: locset) (parent retaddr: val) :=
-  mconj (frame_contents_1 j sp ls ls0 parent retaddr)
+Definition frame_contents (j: meminj) (sp: block) (ls ls0: locset) (parent retaddr: val) (cp: compartment) :=
+  (* let cp := default_compartment in *)
+  mconj (frame_contents_1 j sp ls ls0 parent retaddr cp)
         (range sp 0 fe.(fe_stack_data) **
          range sp (fe.(fe_stack_data) + b.(bound_stack_data)) fe.(fe_size)).
 
 (** Accessing components of the frame. *)
 
 Lemma frame_get_local:
-  forall ofs ty j sp ls ls0 parent retaddr m P,
-  m |= frame_contents j sp ls ls0 parent retaddr ** P ->
+  forall ofs ty j sp ls ls0 parent retaddr cp m P,
+  m |= frame_contents j sp ls ls0 parent retaddr cp ** P ->
   slot_within_bounds b Local ofs ty -> slot_valid f Local ofs ty = true ->
   exists v,
-     load_stack m (Vptr sp Ptrofs.zero) ty (Ptrofs.repr (offset_local fe ofs)) = Some v
+     load_stack m (Vptr sp Ptrofs.zero) ty (Ptrofs.repr (offset_local fe ofs)) cp = Some v
   /\ Val.inject j (ls (S Local ofs ty)) v.
 Proof.
   unfold frame_contents, frame_contents_1; intros. unfold slot_valid in H1; InvBooleans.
@@ -407,11 +438,11 @@ Proof.
 Qed.
 
 Lemma frame_get_outgoing:
-  forall ofs ty j sp ls ls0 parent retaddr m P,
-  m |= frame_contents j sp ls ls0 parent retaddr ** P ->
+  forall ofs ty j sp ls ls0 parent retaddr cp m P,
+  m |= frame_contents j sp ls ls0 parent retaddr cp ** P ->
   slot_within_bounds b Outgoing ofs ty -> slot_valid f Outgoing ofs ty = true ->
   exists v,
-     load_stack m (Vptr sp Ptrofs.zero) ty (Ptrofs.repr (offset_arg ofs)) = Some v
+     load_stack m (Vptr sp Ptrofs.zero) ty (Ptrofs.repr (offset_arg ofs)) cp = Some v
   /\ Val.inject j (ls (S Outgoing ofs ty)) v.
 Proof.
   unfold frame_contents, frame_contents_1; intros. unfold slot_valid in H1; InvBooleans.
@@ -420,9 +451,9 @@ Proof.
 Qed.
 
 Lemma frame_get_parent:
-  forall j sp ls ls0 parent retaddr m P,
-  m |= frame_contents j sp ls ls0 parent retaddr ** P ->
-  load_stack m (Vptr sp Ptrofs.zero) Tptr (Ptrofs.repr fe.(fe_ofs_link)) = Some parent.
+  forall j sp ls ls0 parent retaddr cp m P,
+  m |= frame_contents j sp ls ls0 parent retaddr cp ** P ->
+  load_stack m (Vptr sp Ptrofs.zero) Tptr (Ptrofs.repr fe.(fe_ofs_link)) cp = Some parent.
 Proof.
   unfold frame_contents, frame_contents_1; intros.
   apply mconj_proj1 in H. apply sep_proj1 in H. apply sep_pick3 in H. rewrite <- chunk_of_Tptr in H.
@@ -430,9 +461,9 @@ Proof.
 Qed.
 
 Lemma frame_get_retaddr:
-  forall j sp ls ls0 parent retaddr m P,
-  m |= frame_contents j sp ls ls0 parent retaddr ** P ->
-  load_stack m (Vptr sp Ptrofs.zero) Tptr (Ptrofs.repr fe.(fe_ofs_retaddr)) = Some retaddr.
+  forall j sp ls ls0 parent retaddr cp m P,
+  m |= frame_contents j sp ls ls0 parent retaddr cp ** P ->
+  load_stack m (Vptr sp Ptrofs.zero) Tptr (Ptrofs.repr fe.(fe_ofs_retaddr)) cp = Some retaddr.
 Proof.
   unfold frame_contents, frame_contents_1; intros.
   apply mconj_proj1 in H. apply sep_proj1 in H. apply sep_pick4 in H. rewrite <- chunk_of_Tptr in H.
@@ -442,13 +473,13 @@ Qed.
 (** Assigning a [Local] or [Outgoing] stack slot. *)
 
 Lemma frame_set_local:
-  forall ofs ty v v' j sp ls ls0 parent retaddr m P,
-  m |= frame_contents j sp ls ls0 parent retaddr ** P ->
+  forall ofs ty v v' j sp ls ls0 parent retaddr cp m P,
+  m |= frame_contents j sp ls ls0 parent retaddr cp ** P ->
   slot_within_bounds b Local ofs ty -> slot_valid f Local ofs ty = true ->
   Val.inject j v v' ->
   exists m',
-     store_stack m (Vptr sp Ptrofs.zero) ty (Ptrofs.repr (offset_local fe ofs)) v' = Some m'
-  /\ m' |= frame_contents j sp (Locmap.set (S Local ofs ty) v ls) ls0 parent retaddr ** P.
+     store_stack m (Vptr sp Ptrofs.zero) ty (Ptrofs.repr (offset_local fe ofs)) v' cp = Some m'
+  /\ m' |= frame_contents j sp (Locmap.set (S Local ofs ty) v ls) ls0 parent retaddr cp ** P.
 Proof.
   intros. unfold frame_contents in H.
   exploit mconj_proj1; eauto. unfold frame_contents_1.
@@ -467,13 +498,13 @@ Proof.
 Qed.
 
 Lemma frame_set_outgoing:
-  forall ofs ty v v' j sp ls ls0 parent retaddr m P,
-  m |= frame_contents j sp ls ls0 parent retaddr ** P ->
+  forall ofs ty v v' j sp ls ls0 parent retaddr cp m P,
+  m |= frame_contents j sp ls ls0 parent retaddr cp ** P ->
   slot_within_bounds b Outgoing ofs ty -> slot_valid f Outgoing ofs ty = true ->
   Val.inject j v v' ->
   exists m',
-     store_stack m (Vptr sp Ptrofs.zero) ty (Ptrofs.repr (offset_arg ofs)) v' = Some m'
-  /\ m' |= frame_contents j sp (Locmap.set (S Outgoing ofs ty) v ls) ls0 parent retaddr ** P.
+     store_stack m (Vptr sp Ptrofs.zero) ty (Ptrofs.repr (offset_arg ofs)) v' cp = Some m'
+  /\ m' |= frame_contents j sp (Locmap.set (S Outgoing ofs ty) v ls) ls0 parent retaddr cp ** P.
 Proof.
   intros. unfold frame_contents in H.
   exploit mconj_proj1; eauto. unfold frame_contents_1.
@@ -494,12 +525,12 @@ Qed.
 (** Invariance by change of location maps. *)
 
 Lemma frame_contents_exten:
-  forall ls ls0 ls' ls0' j sp parent retaddr P m,
+  forall ls ls0 ls' ls0' j sp parent retaddr cp P m,
   (forall ofs ty, Val.lessdef (ls' (S Local ofs ty)) (ls (S Local ofs ty))) ->
   (forall ofs ty, Val.lessdef (ls' (S Outgoing ofs ty)) (ls (S Outgoing ofs ty))) ->
   (forall r, In r b.(used_callee_save) -> ls0' (R r) = ls0 (R r)) ->
-  m |= frame_contents j sp ls ls0 parent retaddr ** P ->
-  m |= frame_contents j sp ls' ls0' parent retaddr ** P.
+  m |= frame_contents j sp ls ls0 parent retaddr cp ** P ->
+  m |= frame_contents j sp ls' ls0' parent retaddr cp ** P.
 Proof.
   unfold frame_contents, frame_contents_1; intros.
   rewrite <- ! (contains_locations_exten ls ls') by auto.
@@ -510,17 +541,17 @@ Qed.
 (** Invariance by assignment to registers. *)
 
 Corollary frame_set_reg:
-  forall r v j sp ls ls0 parent retaddr m P,
-  m |= frame_contents j sp ls ls0 parent retaddr ** P ->
-  m |= frame_contents j sp (Locmap.set (R r) v ls) ls0 parent retaddr ** P.
+  forall r v j sp ls ls0 parent retaddr cp m P,
+  m |= frame_contents j sp ls ls0 parent retaddr cp ** P ->
+  m |= frame_contents j sp (Locmap.set (R r) v ls) ls0 parent retaddr cp ** P.
 Proof.
   intros. apply frame_contents_exten with ls ls0; auto.
 Qed.
 
 Corollary frame_undef_regs:
-  forall j sp ls ls0 parent retaddr m P rl,
-  m |= frame_contents j sp ls ls0 parent retaddr ** P ->
-  m |= frame_contents j sp (LTL.undef_regs rl ls) ls0 parent retaddr ** P.
+  forall j sp ls ls0 parent retaddr cp m P rl,
+  m |= frame_contents j sp ls ls0 parent retaddr cp ** P ->
+  m |= frame_contents j sp (LTL.undef_regs rl ls) ls0 parent retaddr cp ** P.
 Proof.
 Local Opaque sepconj.
   induction rl; simpl; intros.
@@ -529,9 +560,9 @@ Local Opaque sepconj.
 Qed.
 
 Corollary frame_set_regpair:
-  forall j sp ls0 parent retaddr m P p v ls,
-  m |= frame_contents j sp ls ls0 parent retaddr ** P ->
-  m |= frame_contents j sp (Locmap.setpair p v ls) ls0 parent retaddr ** P.
+  forall j sp ls0 parent retaddr cp m P p v ls,
+  m |= frame_contents j sp ls ls0 parent retaddr cp ** P ->
+  m |= frame_contents j sp (Locmap.setpair p v ls) ls0 parent retaddr cp ** P.
 Proof.
   intros. destruct p; simpl.
   apply frame_set_reg; auto.
@@ -539,9 +570,9 @@ Proof.
 Qed.
 
 Corollary frame_set_res:
-  forall j sp ls0 parent retaddr m P res v ls,
-  m |= frame_contents j sp ls ls0 parent retaddr ** P ->
-  m |= frame_contents j sp (Locmap.setres res v ls) ls0 parent retaddr ** P.
+  forall j sp ls0 parent retaddr cp m P res v ls,
+  m |= frame_contents j sp ls ls0 parent retaddr cp ** P ->
+  m |= frame_contents j sp (Locmap.setres res v ls) ls0 parent retaddr cp ** P.
 Proof.
   induction res; simpl; intros.
 - apply frame_set_reg; auto.
@@ -552,10 +583,10 @@ Qed.
 (** Invariance by change of memory injection. *)
 
 Lemma frame_contents_incr:
-  forall j sp ls ls0 parent retaddr m P j',
-  m |= frame_contents j sp ls ls0 parent retaddr ** P ->
+  forall j sp ls ls0 parent retaddr cp m P j',
+  m |= frame_contents j sp ls ls0 parent retaddr cp ** P ->
   inject_incr j j' ->
-  m |= frame_contents j' sp ls ls0 parent retaddr ** P.
+  m |= frame_contents j' sp ls ls0 parent retaddr cp ** P.
 Proof.
   unfold frame_contents, frame_contents_1; intros.
   rewrite <- (contains_locations_incr j j') by auto.
@@ -917,15 +948,16 @@ Hypothesis ls_temp_undef:
 Hypothesis wt_ls: forall r, Val.has_type (ls (R r)) (mreg_type r).
 
 Lemma save_callee_save_rec_correct:
-  forall k l pos rs m P,
+  forall k l pos cp rs m P,
   (forall r, In r l -> is_callee_save r = true) ->
   m |= range sp pos (size_callee_save_area_rec l pos) ** P ->
+  forall OWN : Mem.own_block m sp cp,
   agree_regs j ls rs ->
   exists rs', exists m',
      star (step tpol) tge
         (State cs fb (Vptr sp Ptrofs.zero) (save_callee_save_rec l pos k) rs m)
      E0 (State cs fb (Vptr sp Ptrofs.zero) k rs' m')
-  /\ m' |= contains_callee_saves j sp pos l ls ** P
+  /\ m' |= contains_callee_saves j sp pos l ls cp ** P
   /\ (forall ofs k p, Mem.perm m sp ofs k p -> Mem.perm m' sp ofs k p)
   /\ agree_regs j ls rs'.
 Proof.
@@ -949,25 +981,31 @@ Local Opaque mreg_type.
   apply range_drop_left with (mid := pos1) in SEP; [ | omega ].
   apply range_split with (mid := pos1 + sz) in SEP; [ | omega ].
   unfold sz at 1 in SEP. rewrite <- size_type_chunk in SEP.
-  apply range_contains in SEP; auto.
+  eapply range_contains in SEP; eauto.
   exploit (contains_set_stack (fun v' => Val.inject j (ls (R r)) v') (rs r)).
   eexact SEP.
-  apply load_result_inject; auto. apply wt_ls.
+  admit. (* RB: NOTE: [Val.inject] on [load_result] (now) fails *)
+  (* eapply load_result_inject; eauto. apply wt_ls. *)
   clear SEP; intros (m1 & STORE & SEP).
   set (rs1 := undef_regs (destroyed_by_setstack ty) rs).
   assert (AG1: agree_regs j ls rs1).
   { red; intros. unfold rs1. destruct (In_dec mreg_eq r0 (destroyed_by_setstack ty)).
     erewrite ls_temp_undef by eauto. auto.
-    rewrite undef_regs_other by auto. apply AG. }
+    rewrite undef_regs_other by auto.
+    admit. (* RB: NOTE: [Val.inject] (now) fails *)
+    (* apply AG. *)
+  }
   rewrite sep_swap in SEP.
-  exploit (IHl (pos1 + sz) rs1 m1); eauto.
+  exploit (IHl (pos1 + sz) cp rs1 m1); eauto.
+  admit. (* RB: NOTE: New own_block subgoal *)
   intros (rs2 & m2 & A & B & C & D).
   exists rs2, m2.
-  split. eapply star_left; eauto. constructor. exact STORE. auto. traceEq.
+  split. eapply star_left; eauto. econstructor. exact STORE. auto. traceEq.
   split. rewrite sep_assoc, sep_swap. exact B.
   split. intros. apply C. unfold store_stack in STORE; simpl in STORE. eapply Mem.perm_store_1; eauto.
   auto.
-Qed.
+(* Qed. *)
+Admitted.
 
 End SAVE_CALLEE_SAVE.
 
@@ -1005,7 +1043,7 @@ Proof.
 Qed.
 
 Lemma save_callee_save_correct:
-  forall j ls ls0 rs sp cs fb k m P,
+  forall j ls ls0 rs sp cs fb k cp m P,
   m |= range sp fe.(fe_ofs_callee_save) (size_callee_save_area b fe.(fe_ofs_callee_save)) ** P ->
   (forall r, Val.has_type (ls (R r)) (mreg_type r)) ->
   agree_callee_save ls ls0 ->
@@ -1016,7 +1054,7 @@ Lemma save_callee_save_correct:
      star (step tpol) tge
         (State cs fb (Vptr sp Ptrofs.zero) (save_callee_save fe k) rs1 m)
      E0 (State cs fb (Vptr sp Ptrofs.zero) k rs' m')
-  /\ m' |= contains_callee_saves j sp fe.(fe_ofs_callee_save) b.(used_callee_save) ls0 ** P
+  /\ m' |= contains_callee_saves j sp fe.(fe_ofs_callee_save) b.(used_callee_save) ls0 cp ** P
   /\ (forall ofs k p, Mem.perm m sp ofs k p -> Mem.perm m' sp ofs k p)
   /\ agree_regs j ls1 rs'.
 Proof.
@@ -1026,6 +1064,7 @@ Proof.
 - intros. unfold ls1. apply undef_regs_type. apply TY.
 - exact b.(used_callee_save_prop).
 - eexact SEP.
+- admit. (* RB: NOTE: New own_block subgoal *)
 - instantiate (1 := rs1). apply agree_regs_undef_regs. apply agree_regs_call_regs. auto.
 - clear SEP. intros (rs' & m' & EXEC & SEP & PERMS & AG').
   exists rs', m'.
@@ -1041,12 +1080,25 @@ Proof.
     { apply existsb_exists. exists r; auto. }
     congruence.
   split. exact PERMS. exact AG'.
-Qed.
+(* Qed. *)
+Admitted.
 
 (** As a corollary of the previous lemmas, we obtain the following
   correctness theorem for the execution of a function prologue
   (allocation of the frame + saving of the link and return address +
   saving of the used callee-save registers). *)
+
+(* RB: NOTE: Where should this remark live? Interestingly, with the addition of
+   component-based access the next lemma needs this equality explicitly. *)
+Remark transf_function_comp:
+  Linear.fn_comp f = fn_comp tf.
+Proof.
+  unfold transf_function in TRANSF_F.
+  destruct (negb (wt_function f));
+    destruct (zlt Ptrofs.max_unsigned (fe_size (make_env (function_bounds f))));
+    inversion TRANSF_F.
+  reflexivity.
+Qed.
 
 Lemma function_prologue_correct:
   forall j ls ls0 ls1 rs rs1 m1 m1' m2 sp parent ra cs fb k P,
@@ -1061,14 +1113,14 @@ Lemma function_prologue_correct:
   m1' |= minjection j m1 ** globalenv_inject ge j ** P ->
   exists j', exists rs', exists m2', exists sp', exists m3', exists m4', exists m5',
      Mem.alloc m1' tf.(fn_comp) 0 tf.(fn_stacksize) = (m2', sp')
-  /\ store_stack m2' (Vptr sp' Ptrofs.zero) Tptr tf.(fn_link_ofs) parent = Some m3'
-  /\ store_stack m3' (Vptr sp' Ptrofs.zero) Tptr tf.(fn_retaddr_ofs) ra = Some m4'
+  /\ store_stack m2' (Vptr sp' Ptrofs.zero) Tptr tf.(fn_link_ofs) parent tf.(fn_comp) = Some m3'
+  /\ store_stack m3' (Vptr sp' Ptrofs.zero) Tptr tf.(fn_retaddr_ofs) ra tf.(fn_comp) = Some m4'
   /\ star (step tpol) tge
          (State cs fb (Vptr sp' Ptrofs.zero) (save_callee_save fe k) rs1 m4')
       E0 (State cs fb (Vptr sp' Ptrofs.zero) k rs' m5')
   /\ agree_regs j' ls1 rs'
   /\ agree_locs ls1 ls0
-  /\ m5' |= frame_contents j' sp' ls1 ls0 parent ra ** minjection j' m2 ** globalenv_inject ge j' ** P
+  /\ m5' |= frame_contents j' sp' ls1 ls0 parent ra tf.(fn_comp) ** minjection j' m2 ** globalenv_inject ge j' ** P
   /\ j' sp = Some(sp', fe.(fe_stack_data))
   /\ inject_incr j j'.
 Proof.
@@ -1100,14 +1152,16 @@ Local Opaque b fe.
   apply (frame_env_separated b) in SEP. replace (make_env b) with fe in SEP by auto.
   (* Store of parent *)
   rewrite sep_swap3 in SEP.
-  apply (range_contains Mptr) in SEP; [|tauto].
+  eapply (range_contains Mptr) in SEP; [|tauto
+                                        |admit]. (* RB: NOTE: New own_block subgoal *)
   exploit (contains_set_stack (fun v' => v' = parent) parent (fun _ => True) m2' Tptr).
   rewrite chunk_of_Tptr; eexact SEP. apply Val.load_result_same; auto.
   clear SEP; intros (m3' & STORE_PARENT & SEP).
   rewrite sep_swap3 in SEP.
   (* Store of return address *)
   rewrite sep_swap4 in SEP.
-  apply (range_contains Mptr) in SEP; [|tauto].
+  eapply (range_contains Mptr) in SEP; [|tauto
+                                        |admit]. (* RB: NOTE: New own_block subgoal *)
   exploit (contains_set_stack (fun v' => v' = ra) ra (fun _ => True) m3' Tptr).
   rewrite chunk_of_Tptr; eexact SEP. apply Val.load_result_same; auto.
   clear SEP; intros (m4' & STORE_RETADDR & SEP).
@@ -1132,7 +1186,7 @@ Local Opaque b fe.
   clear SEP; intros SEP.
   rewrite sep_swap in SEP.
   (* Now we frame this *)
-  assert (SEPFINAL: m5' |= frame_contents j' sp' ls1 ls0 parent ra ** minjection j' m2 ** globalenv_inject ge j' ** P).
+  assert (SEPFINAL: m5' |= frame_contents j' sp' ls1 ls0 parent ra tf.(fn_comp) ** minjection j' m2 ** globalenv_inject ge j' ** P).
   { eapply frame_mconj. eexact SEPCONJ.
     rewrite chunk_of_Tptr in SEP.
     unfold frame_contents_1; rewrite ! sep_assoc. exact SEP.
@@ -1148,6 +1202,7 @@ Local Opaque b fe.
   clear SEP SEPCONJ.
 (* Conclusions *)
   exists j', rs2, m2', sp', m3', m4', m5'.
+  rewrite transf_function_comp in *.
   split. auto.
   split. exact STORE_PARENT.
   split. exact STORE_RETADDR.
@@ -1159,7 +1214,8 @@ Local Opaque b fe.
     unfold call_regs. apply AGARGS. apply incoming_slot_in_parameters; auto.
   split. exact SEPFINAL.
   split. exact SAME. exact INCR.
-Qed.
+(* Qed. *)
+Admitted.
 
 (** The following lemmas show the correctness of the register reloading
   code generated by [reload_callee_save]: after this code has executed,
@@ -1179,8 +1235,8 @@ Definition agree_unused (ls0: locset) (rs: regset) : Prop :=
   forall r, ~(mreg_within_bounds b r) -> Val.inject j (ls0 (R r)) (rs r).
 
 Lemma restore_callee_save_rec_correct:
-  forall l ofs rs k,
-  m |= contains_callee_saves j sp ofs l ls0 ->
+  forall l ofs cp rs k,
+  m |= contains_callee_saves j sp ofs l ls0 cp ->
   agree_unused ls0 rs ->
   (forall r, In r l -> mreg_within_bounds b r) ->
   exists rs',
@@ -1205,7 +1261,7 @@ Local Opaque mreg_type.
   exploit contains_get_stack.
     eapply sep_proj1; eassumption.
   intros (v & LOAD & SPEC).
-  exploit (IHl (ofs1 + sz) (rs#r <- v)).
+  exploit (IHl (ofs1 + sz) cp (rs#r <- v)).
     eapply sep_proj2; eassumption.
     red; intros. rewrite Regmap.gso. auto. intuition congruence.
     eauto.
@@ -1225,8 +1281,8 @@ Qed.
 End RESTORE_CALLEE_SAVE.
 
 Lemma restore_callee_save_correct:
-  forall m j sp ls ls0 pa ra P rs k cs fb,
-  m |= frame_contents j sp ls ls0 pa ra ** P ->
+  forall m j sp ls ls0 pa ra cp P rs k cs fb,
+  m |= frame_contents j sp ls ls0 pa ra cp ** P ->
   agree_unused j ls0 rs ->
   exists rs',
     star (step tpol) tge
@@ -1258,16 +1314,16 @@ Qed.
   of the frame). *)
 
 Lemma function_epilogue_correct:
-  forall m' j sp' ls ls0 pa ra P m rs sp m1 k cs fb,
-  m' |= frame_contents j sp' ls ls0 pa ra ** minjection j m ** P ->
+  forall m' j sp' cp' ls ls0 pa ra P m rs sp cp m1 k cs fb,
+    m' |= frame_contents j sp' ls ls0 pa ra cp' ** minjection j m ** P ->
   agree_regs j ls rs ->
   agree_locs ls ls0 ->
   j sp = Some(sp', fe.(fe_stack_data)) ->
-  Mem.free m sp 0 f.(Linear.fn_stacksize) = Some m1 ->
+  Mem.free m sp 0 f.(Linear.fn_stacksize) cp = Some m1 ->
   exists rs1, exists m1',
-     load_stack m' (Vptr sp' Ptrofs.zero) Tptr tf.(fn_link_ofs) = Some pa
-  /\ load_stack m' (Vptr sp' Ptrofs.zero) Tptr tf.(fn_retaddr_ofs) = Some ra
-  /\ Mem.free m' sp' 0 tf.(fn_stacksize) = Some m1'
+     load_stack m' (Vptr sp' Ptrofs.zero) Tptr tf.(fn_link_ofs) cp' = Some pa
+  /\ load_stack m' (Vptr sp' Ptrofs.zero) Tptr tf.(fn_retaddr_ofs) cp' = Some ra
+  /\ Mem.free m' sp' 0 tf.(fn_stacksize) cp' = Some m1'
   /\ star (step tpol) tge
        (State cs fb (Vptr sp' Ptrofs.zero) (restore_callee_save fe k) rs m')
     E0 (State cs fb (Vptr sp' Ptrofs.zero) k rs1 m')
@@ -1300,7 +1356,7 @@ Proof.
   exists rs', m1'.
   split. assumption.
   split. assumption.
-  split. assumption.
+  split. (*assumption.*) admit. (* RB: NOTE: Cross-operation component determinacy *)
   split. eassumption.
   split. red; unfold return_regs; intros.
     destruct (is_callee_save r) eqn:C.
@@ -1309,7 +1365,8 @@ Proof.
   split. red; unfold return_regs; intros.
     destruct l. rewrite H; auto. destruct sl; auto; contradiction. 
   assumption.
-Qed.
+(* Qed. *)
+Admitted.
 
 End FRAME_PROPERTIES.
 
@@ -1318,12 +1375,12 @@ End FRAME_PROPERTIES.
 (** This is the memory assertion that captures the contents of the stack frames
   mentioned in the call stacks. *)
 
-Fixpoint stack_contents (j: meminj) (cs: list Linear.stackframe) (cs': list Mach.stackframe) : massert :=
+Fixpoint stack_contents (j: meminj) (cs: list Linear.stackframe) (cs': list Mach.stackframe) (cp: compartment) : massert :=
   match cs, cs' with
   | nil, nil => pure True
   | Linear.Stackframe f _ ls c :: cs, Mach.Stackframe fb (Vptr sp' _) ra c' :: cs' =>
-      frame_contents f j sp' ls (parent_locset cs) (parent_sp cs') (parent_ra cs')
-      ** stack_contents j cs cs'
+      frame_contents f j sp' ls (parent_locset cs) (parent_sp cs') (parent_ra cs') cp
+      ** stack_contents j cs cs' cp
   | _, _ => pure False
   end.
 
@@ -1357,9 +1414,9 @@ Inductive match_stacks (j: meminj):
 
 Lemma stack_contents_change_meminj:
   forall m j j', inject_incr j j' ->
-  forall cs cs' P,
-  m |= stack_contents j cs cs' ** P ->
-  m |= stack_contents j' cs cs' ** P.
+  forall cs cs' cp P,
+  m |= stack_contents j cs cs' cp ** P ->
+  m |= stack_contents j' cs cs' cp ** P.
 Proof.
 Local Opaque sepconj.
   induction cs as [ | [] cs]; destruct cs' as [ | [] cs']; simpl; intros; auto.
@@ -1548,18 +1605,18 @@ Qed.
 
 Lemma symbols_preserved:
   forall (s: ident), Genv.find_symbol tge s = Genv.find_symbol ge s.
-Proof (Genv.find_symbol_match TRANSF).
+Proof. exact (Genv.find_symbol_match TRANSF). Qed.
 
 Lemma senv_preserved:
   Senv.equiv ge tge.
-Proof (Genv.senv_match TRANSF).
+Proof. exact (Genv.senv_match TRANSF). Qed.
 
 Lemma functions_translated:
   forall v f,
   Genv.find_funct ge v = Some f ->
   exists tf,
   Genv.find_funct tge v = Some tf /\ transf_fundef f = OK tf.
-Proof (Genv.find_funct_transf_partial TRANSF).
+Proof. exact (Genv.find_funct_transf_partial TRANSF). Qed.
 
 Lemma function_ptr_translated:
   forall b f,
@@ -1617,7 +1674,8 @@ Hypothesis AGR: agree_regs j ls rs.
 Hypothesis AGCS: agree_callee_save ls (parent_locset cs).
 Hypothesis AGARGS: agree_outgoing_arguments sg ls (parent_locset cs).
 Variable m': mem.
-Hypothesis SEP: m' |= stack_contents j cs cs'.
+Variable cp: compartment.
+Hypothesis SEP: m' |= stack_contents j cs cs' cp.
 
 Lemma transl_external_argument:
   forall l,
@@ -1638,7 +1696,7 @@ Proof.
   assert (slot_within_bounds (function_bounds f) Outgoing pos ty) by eauto.
   exploit frame_get_outgoing; eauto. intros (v & A & B).
   exists v; split.
-  constructor. exact A. rewrite AGARGS by auto. exact B. 
+  econstructor. exact A. rewrite AGARGS by auto. exact B.
 Qed.
 
 Lemma transl_external_argument_2:
@@ -1699,7 +1757,8 @@ Variables sp sp': block.
 Variables parent retaddr: val.
 Hypothesis INJ: j sp = Some(sp', fe.(fe_stack_data)).
 Hypothesis AGR: agree_regs j ls rs.
-Hypothesis SEP: m' |= frame_contents f j sp' ls ls0 parent retaddr ** minjection j m ** globalenv_inject ge j.
+Variable cp: compartment.
+Hypothesis SEP: m' |= frame_contents f j sp' ls ls0 parent retaddr cp ** minjection j m ** globalenv_inject ge j.
 
 Lemma transl_builtin_arg_correct:
   forall a v,
@@ -1722,7 +1781,7 @@ Local Opaque fe.
   destruct x as [r | [] ofs ty]; try discriminate.
   + exists (rs r); auto with barg.
   + exploit frame_get_local; eauto. intros (v & A & B).
-    exists v; split; auto. constructor; auto.
+    exists v; split; auto. econstructor; eauto.
 - econstructor; eauto with barg.
 - econstructor; eauto with barg.
 - econstructor; eauto with barg.
@@ -1731,11 +1790,11 @@ Local Opaque fe.
   apply sep_proj2 in SEP. apply sep_proj1 in SEP. exploit loadv_parallel_rule; eauto.
   instantiate (1 := Val.offset_ptr (Vptr sp' Ptrofs.zero) ofs').
   simpl. rewrite ! Ptrofs.add_zero_l. econstructor; eauto.
-  intros (v' & A & B). exists v'; split; auto. constructor; auto.
+  intros (v' & A & B). exists v'; split; auto. econstructor; eauto.
 - econstructor; split; eauto with barg.
   unfold Val.offset_ptr. rewrite ! Ptrofs.add_zero_l. econstructor; eauto.
 - apply sep_proj2 in SEP. apply sep_proj1 in SEP. exploit loadv_parallel_rule; eauto.
-  intros (v' & A & B). exists v'; auto with barg.
+  intros (v' & A & B). exists v'; eauto with barg.
 - econstructor; split; eauto with barg.
 - destruct IHeval_builtin_arg1 as (v1 & A1 & B1); auto using in_or_app.
   destruct IHeval_builtin_arg2 as (v2 & A2 & B2); auto using in_or_app.
@@ -1793,7 +1852,7 @@ End BUILTIN_ARGUMENTS.
 
 Inductive match_states: Linear.state -> Mach.state -> Prop :=
   | match_states_intro:
-      forall cs f sp c ls m cs' fb sp' rs m' j tf
+      forall cs f sp c ls m cs' fb sp' rs m' j tf cp
         (STACKS: match_stacks j cs cs' f.(Linear.fn_sig))
         (TRANSL: transf_function f = OK tf)
         (FIND: Genv.find_funct_ptr tge fb = Some (Internal tf))
@@ -1801,28 +1860,28 @@ Inductive match_states: Linear.state -> Mach.state -> Prop :=
         (AGLOCS: agree_locs f ls (parent_locset cs))
         (INJSP: j sp = Some(sp', fe_stack_data (make_env (function_bounds f))))
         (TAIL: is_tail c (Linear.fn_code f))
-        (SEP: m' |= frame_contents f j sp' ls (parent_locset cs) (parent_sp cs') (parent_ra cs')
-                 ** stack_contents j cs cs'
+        (SEP: m' |= frame_contents f j sp' ls (parent_locset cs) (parent_sp cs') (parent_ra cs') cp
+                 ** stack_contents j cs cs' cp
                  ** minjection j m
                  ** globalenv_inject ge j),
       match_states (Linear.State cs f (Vptr sp Ptrofs.zero) c ls m)
                    (Mach.State cs' fb (Vptr sp' Ptrofs.zero) (transl_code (make_env (function_bounds f)) c) rs m')
   | match_states_call:
-      forall cs f ls m cs' fb rs m' j tf
+      forall cs f ls m cs' fb rs m' j tf cp
         (STACKS: match_stacks j cs cs' (Linear.funsig f))
         (TRANSL: transf_fundef f = OK tf)
         (FIND: Genv.find_funct_ptr tge fb = Some (tf))
         (AGREGS: agree_regs j ls rs)
-        (SEP: m' |= stack_contents j cs cs'
+        (SEP: m' |= stack_contents j cs cs' cp
                  ** minjection j m
                  ** globalenv_inject ge j),
       match_states (Linear.Callstate cs f ls m)
                    (Mach.Callstate cs' fb rs m')
   | match_states_return:
-      forall cs ls m cs' rs m' j sg
+      forall cs ls m cs' rs m' j sg cp
         (STACKS: match_stacks j cs cs' sg)
         (AGREGS: agree_regs j ls rs)
-        (SEP: m' |= stack_contents j cs cs'
+        (SEP: m' |= stack_contents j cs cs' cp
                  ** minjection j m
                  ** globalenv_inject ge j),
       match_states (Linear.Returnstate cs ls m)
@@ -1847,10 +1906,11 @@ Proof.
 + (* Lgetstack, local *)
   exploit frame_get_local; eauto. intros (v & A & B).
   econstructor; split.
-  apply plus_one. apply exec_Mgetstack. exact A.
+  apply plus_one. eapply exec_Mgetstack. exact A.
   econstructor; eauto with coqlib.
   apply agree_regs_set_reg; auto.
   apply agree_locs_set_reg; auto.
+  instantiate (1 := cp); auto.
 + (* Lgetstack, incoming *)
   unfold slot_valid in SV. InvBooleans.
   exploit incoming_slot_in_parameters; eauto. intros IN_ARGS.
@@ -1870,13 +1930,15 @@ Proof.
   apply agree_regs_set_reg. apply agree_regs_set_reg. auto. auto.
   erewrite agree_incoming by eauto. exact B.
   apply agree_locs_set_reg; auto. apply agree_locs_undef_locs; auto.
+  instantiate (1 := cp); auto.
 + (* Lgetstack, outgoing *)
   exploit frame_get_outgoing; eauto. intros (v & A & B).
   econstructor; split.
-  apply plus_one. apply exec_Mgetstack. exact A.
+  apply plus_one. eapply exec_Mgetstack. exact A.
   econstructor; eauto with coqlib.
   apply agree_regs_set_reg; auto.
   apply agree_locs_set_reg; auto.
+  instantiate (1 := cp); auto.
 
 - (* Lsetstack *)
   exploit wt_state_setstack; eauto. intros (SV & SW).
@@ -1887,11 +1949,11 @@ Proof.
                end).
   eapply frame_undef_regs with (rl := destroyed_by_setstack ty) in SEP.
   assert (A: exists m'',
-              store_stack m' (Vptr sp' Ptrofs.zero) ty (Ptrofs.repr ofs') (rs0 src) = Some m''
+              store_stack m' (Vptr sp' Ptrofs.zero) ty (Ptrofs.repr ofs') (rs0 src) cp = Some m''
            /\ m'' |= frame_contents f j sp' (Locmap.set (S sl ofs ty) (rs (R src))
                                                (LTL.undef_regs (destroyed_by_setstack ty) rs))
-                                            (parent_locset s) (parent_sp cs') (parent_ra cs')
-                  ** stack_contents j s cs' ** minjection j m ** globalenv_inject ge j).
+                                            (parent_locset s) (parent_sp cs') (parent_ra cs') cp
+                  ** stack_contents j s cs' cp ** minjection j m ** globalenv_inject ge j).
   { unfold ofs'; destruct sl; try discriminate.
     eapply frame_set_local; eauto.
     eapply frame_set_outgoing; eauto. }
@@ -1943,6 +2005,7 @@ Proof.
   econstructor; eauto with coqlib.
   apply agree_regs_set_reg. rewrite transl_destroyed_by_load. apply agree_regs_undef_regs; auto. auto.
   apply agree_locs_set_reg. apply agree_locs_undef_locs. auto. apply destroyed_by_load_caller_save. auto.
+  instantiate (1 := cp0); auto.
 
 - (* Lstore *)
   assert (exists a',
@@ -1986,7 +2049,7 @@ Proof.
   simpl. rewrite sep_assoc. exact SEP.
 
 - (* Ltailcall *)
-  rewrite (sep_swap (stack_contents j s cs')) in SEP.
+  rewrite (sep_swap (stack_contents j s cs' cp0)) in SEP.
   exploit function_epilogue_correct; eauto.
   clear SEP. intros (rs1 & m1' & P & Q & R & S & T & U & SEP).
   rewrite sep_swap in SEP.
@@ -2052,6 +2115,7 @@ Proof.
   auto.
   eapply find_label_tail; eauto.
   apply frame_undef_regs; auto.
+  instantiate (1 := cp); auto.
 
 - (* Lcond, false *)
   econstructor; split.
@@ -2062,6 +2126,7 @@ Proof.
   apply agree_locs_undef_locs. auto. apply destroyed_by_cond_caller_save.
   auto. eauto with coqlib.
   apply frame_undef_regs; auto.
+  instantiate (1 := cp); auto.
 
 - (* Ljumptable *)
   assert (rs0 arg = Vint n).
@@ -2074,9 +2139,10 @@ Proof.
   apply agree_locs_undef_locs. auto. apply destroyed_by_jumptable_caller_save.
   auto. eapply find_label_tail; eauto.
   apply frame_undef_regs; auto.
+  instantiate (1 := cp); auto.
 
 - (* Lreturn *)
-  rewrite (sep_swap (stack_contents j s cs')) in SEP.
+  rewrite (sep_swap (stack_contents j s cs' cp0)) in SEP.
   exploit function_epilogue_correct; eauto.
   intros (rs' & m1' & A & B & C & D & E & F & G).
   econstructor; split.
@@ -2105,6 +2171,7 @@ Proof.
   eapply match_states_intro with (j := j'); eauto with coqlib.
   eapply match_stacks_change_meminj; eauto.
   rewrite sep_swap in SEP. rewrite sep_swap. eapply stack_contents_change_meminj; eauto.
+  admit. (* RB: NOTE: Need to connect [cp] and [(fn_comp tfn)] *)
 
 - (* external function *)
   simpl in TRANSL. inversion TRANSL; subst tf.
@@ -2124,6 +2191,7 @@ Proof.
   auto.
   apply stack_contents_change_meminj with j; auto.
   rewrite sep_comm, sep_assoc; auto.
+  instantiate (1 := cp); auto.
 
 - (* return *)
   inv STACKS. exploit wt_returnstate_agree; eauto. intros [AGCS OUTU].
@@ -2135,7 +2203,9 @@ Proof.
   apply frame_contents_exten with rs0 (parent_locset s); auto.
   intros; apply Val.lessdef_same; apply AGCS; red; congruence.
   intros; rewrite (OUTU ty ofs); auto. 
-Qed.
+  instantiate (1 := cp); auto.
+(* Qed. *)
+Admitted.
 
 Lemma transf_initial_states:
   forall st1, Linear.initial_state prog st1 ->
@@ -2162,7 +2232,9 @@ Proof.
     change (Mem.valid_block m0 b0). eapply Genv.find_funct_ptr_not_fresh; eauto.
     change (Mem.valid_block m0 b0). eapply Genv.find_var_info_not_fresh; eauto.
   red; simpl; tauto.
-Qed.
+  Unshelve. (* exact default_compartment.*) admit. (* RB: NOTE: Address disconnected compartment. *)
+(* Qed. *)
+Admitted.
 
 Lemma transf_final_states:
   forall st1 st2 r,
